more

lean/hhg/AExp.java
@@ -1,0 +1,20 @@
+public interface AExp {}
+
+class Num implements AExp {
+    public int num;
+    public Num (int num) { this.num = num; }
+}
+
+class Var implements AExp {
+    public String var;
+    public Var(String var) { this.var = var; }
+}
+
+class Add implements AExp {
+    public AExp left;
+    public AExp right;
+    public Add(AExp left, AExp right)
+        { this.left = left; this.right = right; }
+}
+
+// ....
