lean/hhg/constant.lean
@@ -1,0 +1,13 @@
+constants a b : ℤ
+constant f : ℤ → ℤ
+constant g : ℤ → ℤ → ℤ
+
+--#check λ x : ℤ, g (f (g a x)) (g x b)
+--#check λ x, g (f (g a x)) (g x b)
+
+constant Trool : Type
+constants Trool.true Trool.false Trool.maybe : Trool
+
+
+
+
