lean/hhg/nat.lean
@@ -1,0 +1,14 @@
+inductive nat2 : Type
+| zero : nat2
+| succ : nat2 -> nat2
+
+--#print nat2
+
+inductive aexp : Type
+| num : nat -> aexp         -- TODO: need Z
+| var : string -> aexp
+| add : aexp -> aexp -> aexp
+| sub : aexp -> aexp -> aexp
+| mul : aexp -> aexp -> aexp
+| div : aexp -> aexp -> aexp
+
